theories/SSubst.v
@@ -26,9 +26,17 @@ Fixpoint lift n k t : term :=
   | vnil A => vnil (lift n k A)
   | vcons A a m v => vcons (lift n k A) (lift n k a) (lift n k m) (lift n k v)
   | elim_vec A P e c m v =>
-    elim_vec (lift n k A) (lift n k P)
-             (lift n k e) (lift n k c) (lift n k m) (lift n k v)
+    elim_vec
+      (lift n k A) (lift n k P)
+      (lift n k e) (lift n k c) (lift n k m) (lift n k v)
   | Vec A m => Vec (lift n k A) (lift n k m)
+  | refl A u => refl (lift n k A) (lift n k u)
+  | coe A P u v e t =>
+    coe
+      (lift n k A) (lift n k P)
+      (lift n k u) (lift n k v) (lift n k e)
+      (lift n k t)
+  | Eq A u v => Eq (lift n k A) (lift n k u) (lift n k v)
   | univ s => univ s
   end.
 
@@ -61,6 +69,13 @@ Fixpoint subst s k u :=
     elim_vec (subst s k A) (subst s k P)
              (subst s k e) (subst s k c) (subst s k m) (subst s k v)
   | Vec A m => Vec (subst s k A) (subst s k m)
+  | refl A u => refl (subst s k A) (subst s k u)
+  | coe A P u v e t =>
+    coe
+      (subst s k A) (subst s k P)
+      (subst s k u) (subst s k v) (subst s k e)
+      (subst s k t)
+  | Eq A u v => Eq (subst s k A) (subst s k u) (subst s k v)
   | univ s => univ s
   end.
 
